automation: add structural matcher normalization and integration

Micro_Rust_Parser_Experiment/Micro_Rust_Parser_Cycle_3_Audit.thy
@@ -1,5 +1,7 @@
 theory Micro_Rust_Parser_Cycle_3_Audit
-  imports Micro_Rust_Parser_Cycle_2_Audit
+  imports
+    Micro_Rust_Parser_Cycle_2_Audit
+    Micro_Rust_Parser_Integration
 begin
 
 section\<open> Cycle 3 integration audit \<close>
@@ -44,22 +46,34 @@ where
   \<open> cycle3_some_nineteen = Some 19 \<close>
 
 definition cycle3_some_seven_expression ::
-  \<open>(unit, nat option, unit, unit, unit, unit) expression\<close>
+  \<open>
+    (unit, nat option, nat, unit,
+      unit prompt, unit prompt_output) expression
+  \<close>
 where
   \<open> cycle3_some_seven_expression = literal cycle3_some_seven \<close>
 
 definition cycle3_none_expression ::
-  \<open>(unit, nat option, unit, unit, unit, unit) expression\<close>
+  \<open>
+    (unit, nat option, nat, unit,
+      unit prompt, unit prompt_output) expression
+  \<close>
 where
   \<open> cycle3_none_expression = literal cycle3_none \<close>
 
 definition cycle3_some_three_expression ::
-  \<open>(unit, nat option, unit, unit, unit, unit) expression\<close>
+  \<open>
+    (unit, nat option, nat, unit,
+      unit prompt, unit prompt_output) expression
+  \<close>
 where
   \<open> cycle3_some_three_expression = literal cycle3_some_three \<close>
 
 definition cycle3_single_nine_expression ::
-  \<open>(unit, cycle3_single, unit, unit, unit, unit) expression\<close>
+  \<open>
+    (unit, cycle3_single, nat, unit,
+      unit prompt, unit prompt_output) expression
+  \<close>
 where
   \<open>
     cycle3_single_nine_expression =
@@ -69,7 +83,7 @@ where
 definition cycle3_nested_bits_expression ::
   \<open>
     (unit, cycle3_bit \<times> (cycle3_bit \<times> tnil),
-      unit, unit, unit, unit) expression
+      nat, unit, unit prompt, unit prompt_output) expression
   \<close>
 where
   \<open>
@@ -78,7 +92,10 @@ where
   \<close>
 
 definition cycle3_some_nineteen_expression ::
-  \<open>(unit, nat option, unit, unit, unit, unit) expression\<close>
+  \<open>
+    (unit, nat option, nat, unit,
+      unit prompt, unit prompt_output) expression
+  \<close>
 where
   \<open>
     cycle3_some_nineteen_expression =
@@ -86,7 +103,10 @@ where
   \<close>
 
 definition cycle3_false_expression ::
-  \<open>(unit, bool, unit, unit, unit, unit) expression\<close>
+  \<open>
+    (unit, bool, nat, unit,
+      unit prompt, unit prompt_output) expression
+  \<close>
 where
   \<open> cycle3_false_expression = literal False \<close>
 
@@ -137,27 +157,42 @@ urust_expr cycle3_code_lazy_undefined
   \<close>
 
 definition cycle3_code_constructor_closed ::
-  \<open>(unit, nat, unit, unit, unit, unit) expression\<close>
+  \<open>
+    (unit, nat, nat, unit,
+      unit prompt, unit prompt_output) expression
+  \<close>
 where
   \<open> cycle3_code_constructor_closed = cycle3_code_constructor \<close>
 
 definition cycle3_code_fallthrough_closed ::
-  \<open>(unit, nat, unit, unit, unit, unit) expression\<close>
+  \<open>
+    (unit, nat, nat, unit,
+      unit prompt, unit prompt_output) expression
+  \<close>
 where
   \<open> cycle3_code_fallthrough_closed = cycle3_code_fallthrough \<close>
 
 definition cycle3_code_false_guard_closed ::
-  \<open>(unit, nat, unit, unit, unit, unit) expression\<close>
+  \<open>
+    (unit, nat, nat, unit,
+      unit prompt, unit prompt_output) expression
+  \<close>
 where
   \<open> cycle3_code_false_guard_closed = cycle3_code_false_guard \<close>
 
 definition cycle3_code_exhaustive_closed ::
-  \<open>(unit, nat, unit, unit, unit, unit) expression\<close>
+  \<open>
+    (unit, nat, nat, unit,
+      unit prompt, unit prompt_output) expression
+  \<close>
 where
   \<open> cycle3_code_exhaustive_closed = cycle3_code_exhaustive \<close>
 
 definition cycle3_code_nested_product_or_closed ::
-  \<open>(unit, nat, unit, unit, unit, unit) expression\<close>
+  \<open>
+    (unit, nat, nat, unit,
+      unit prompt, unit prompt_output) expression
+  \<close>
 where
   \<open>
     cycle3_code_nested_product_or_closed =
@@ -165,7 +200,10 @@ where
   \<close>
 
 definition cycle3_code_lazy_undefined_closed ::
-  \<open>(unit, nat, unit, unit, unit, unit) expression\<close>
+  \<open>
+    (unit, nat, nat, unit,
+      unit prompt, unit prompt_output) expression
+  \<close>
 where
   \<open>
     cycle3_code_lazy_undefined_closed =
@@ -173,52 +211,368 @@ where
   \<close>
 
 lemma cycle3_code_constructor_result:
-  \<open> evaluate cycle3_code_constructor_closed () = Success 7 () \<close>
+  \<open>
+    (case evaluate cycle3_code_constructor_closed () of
+       Success value _ \<Rightarrow> value
+     | _ \<Rightarrow> 0) = 7
+  \<close>
   by eval
 
 lemma cycle3_code_fallthrough_result:
-  \<open> evaluate cycle3_code_fallthrough_closed () = Success 11 () \<close>
+  \<open>
+    (case evaluate cycle3_code_fallthrough_closed () of
+       Success value _ \<Rightarrow> value
+     | _ \<Rightarrow> 0) = 11
+  \<close>
   by eval
 
 lemma cycle3_code_false_guard_result:
-  \<open> evaluate cycle3_code_false_guard_closed () = Success 3 () \<close>
+  \<open>
+    (case evaluate cycle3_code_false_guard_closed () of
+       Success value _ \<Rightarrow> value
+     | _ \<Rightarrow> 0) = 3
+  \<close>
   by eval
 
 lemma cycle3_code_exhaustive_result:
-  \<open> evaluate cycle3_code_exhaustive_closed () = Success 9 () \<close>
+  \<open>
+    (case evaluate cycle3_code_exhaustive_closed () of
+       Success value _ \<Rightarrow> value
+     | _ \<Rightarrow> 0) = 9
+  \<close>
   by eval
 
 lemma cycle3_code_nested_product_or_result:
   \<open>
-    evaluate cycle3_code_nested_product_or_closed () =
-      Success 23 ()
+    (case evaluate cycle3_code_nested_product_or_closed () of
+       Success value _ \<Rightarrow> value
+     | _ \<Rightarrow> 0) = 23
   \<close>
   by eval
 
 lemma cycle3_code_lazy_undefined_result:
   \<open>
-    evaluate cycle3_code_lazy_undefined_closed () =
-      Success 19 ()
+    (case evaluate cycle3_code_lazy_undefined_closed () of
+       Success value _ \<Rightarrow> value
+     | _ \<Rightarrow> 0) = 19
   \<close>
   by eval
 
 value [code]
-  \<open> evaluate cycle3_code_constructor_closed () \<close>
+  \<open>
+    case evaluate cycle3_code_constructor_closed () of
+      Success value _ \<Rightarrow> value
+    | _ \<Rightarrow> 0
+  \<close>
 
 value [code]
-  \<open> evaluate cycle3_code_fallthrough_closed () \<close>
+  \<open>
+    case evaluate cycle3_code_fallthrough_closed () of
+      Success value _ \<Rightarrow> value
+    | _ \<Rightarrow> 0
+  \<close>
 
 value [code]
-  \<open> evaluate cycle3_code_false_guard_closed () \<close>
+  \<open>
+    case evaluate cycle3_code_false_guard_closed () of
+      Success value _ \<Rightarrow> value
+    | _ \<Rightarrow> 0
+  \<close>
 
 value [code]
-  \<open> evaluate cycle3_code_exhaustive_closed () \<close>
+  \<open>
+    case evaluate cycle3_code_exhaustive_closed () of
+      Success value _ \<Rightarrow> value
+    | _ \<Rightarrow> 0
+  \<close>
 
 value [code]
-  \<open> evaluate cycle3_code_nested_product_or_closed () \<close>
+  \<open>
+    case evaluate cycle3_code_nested_product_or_closed () of
+      Success value _ \<Rightarrow> value
+    | _ \<Rightarrow> 0
+  \<close>
 
 value [code]
-  \<open> evaluate cycle3_code_lazy_undefined_closed () \<close>
+  \<open>
+    case evaluate cycle3_code_lazy_undefined_closed () of
+      Success value _ \<Rightarrow> value
+    | _ \<Rightarrow> 0
+  \<close>
+
+subsection\<open> Supported proof paths \<close>
+
+definition cycle3_parser_function_expression ::
+  \<open>
+    (unit, nat, nat, unit,
+      unit prompt, unit prompt_output) expression
+  \<close>
+where
+  \<open>
+    cycle3_parser_function_expression \<equiv>
+      cycle3_code_constructor
+  \<close>
+
+lemma cycle3_parser_simp_evaluate:
+  \<open>
+    evaluate cycle3_code_constructor_closed () =
+      Success 7 ()
+  \<close>
+  unfolding cycle3_code_constructor_closed_def
+  apply urust_parser_prepare
+  apply (simp only:
+    cycle3_some_seven_expression_def
+    cycle3_some_seven_def)
+  by urust_parser_simp
+
+lemma cycle3_parser_eval_action:
+  \<open>
+    (yield_handler_no_yield,
+      cycle3_parser_function_expression)
+      \<diamondop>\<^sub>v () =
+    {(7, ())}
+  \<close>
+  unfolding cycle3_parser_function_expression_def
+  apply urust_parser_prepare
+  apply (simp only:
+    cycle3_some_seven_expression_def
+    cycle3_some_seven_def)
+  by urust_parser_simp
+
+lemma cycle3_parser_eval_predicate:
+  \<open>
+    evaluates_to_value yield_handler_no_yield
+      cycle3_parser_function_expression () 7 ()
+  \<close>
+  unfolding cycle3_parser_function_expression_def
+  apply urust_parser_prepare
+  apply (simp only:
+    cycle3_some_seven_expression_def
+    cycle3_some_seven_def)
+  by urust_parser_simp
+
+lemma cycle3_parser_wp:
+  fixes
+    \<Gamma> :: \<open>(unit, unit, unit, unit) striple_context\<close>
+  shows
+    \<open>
+      \<W>\<P> \<Gamma> cycle3_parser_function_expression
+        (\<lambda>_ :: nat. \<top>)
+        (\<lambda>_ :: nat. \<bottom>)
+        (\<lambda>_ :: unit abort. \<bottom>) =
+      \<top>
+  \<close>
+  unfolding cycle3_parser_function_expression_def
+  apply urust_parser_prepare
+  apply (simp only:
+    cycle3_some_seven_expression_def
+    cycle3_some_seven_def)
+  by urust_parser_simp
+
+definition cycle3_parser_function ::
+  \<open>
+    (unit, nat, unit,
+      unit prompt, unit prompt_output) function_body
+  \<close>
+where
+  \<open>
+    cycle3_parser_function \<equiv>
+      FunctionBody cycle3_parser_function_expression
+  \<close>
+
+definition cycle3_parser_contract ::
+  \<open>(unit, nat, unit) function_contract\<close>
+where
+  \<open>
+    cycle3_parser_contract \<equiv>
+      make_function_contract \<top>
+        (\<lambda>result. \<langle>result = 7\<rangle>)
+  \<close>
+
+ucincl_auto cycle3_parser_contract
+
+lemma cycle3_parser_function_contract:
+  fixes
+    \<Gamma> :: \<open>(unit, unit, unit, unit) striple_context\<close>
+  shows
+    \<open>
+      \<Gamma> ; cycle3_parser_function
+        \<Turnstile>\<^sub>F cycle3_parser_contract
+    \<close>
+  apply (crush_boot
+    f: cycle3_parser_function_def
+    contract:
+      cycle3_parser_contract_def)
+  apply (unfold cycle3_parser_function_expression_def)
+  apply urust_parser_prepare
+  by (crush_base simp add:
+    cycle3_some_seven_expression_def
+    cycle3_some_seven_def)
+
+subsection\<open> Controlled-normalization growth \<close>
+
+ML_val\<open>
+  local
+    open Proofterm
+
+    val context = \<^context>
+    val expression_type =
+      \<^typ>\<open>
+        (unit, nat, nat, unit,
+          unit, unit) expression
+      \<close>
+
+    fun audit_assert message condition =
+      if condition then ()
+      else error ("Cycle 3 normalization audit: " ^ message)
+
+    fun proof_nodes MinProof = 1
+      | proof_nodes (PBound _) = 1
+      | proof_nodes (Abst (_, _, proof)) =
+          1 + proof_nodes proof
+      | proof_nodes (AbsP (_, _, proof)) =
+          1 + proof_nodes proof
+      | proof_nodes (proof % _) =
+          1 + proof_nodes proof
+      | proof_nodes (left %% right) =
+          1 + proof_nodes left + proof_nodes right
+      | proof_nodes (Hyp _) = 1
+      | proof_nodes (PAxm _) = 1
+      | proof_nodes (PClass _) = 1
+      | proof_nodes (Oracle _) = 1
+      | proof_nodes (PThm _) = 1
+
+    fun with_recorded_proofs action =
+      let
+        val previous = !Proofterm.proofs
+        val result =
+          Exn.capture
+            (fn () =>
+              (Proofterm.proofs := 2;
+               action ())) ()
+        val _ = Proofterm.proofs := previous
+      in
+        Exn.release result
+      end
+
+    fun marker_name index =
+      "cycle3_source_marker_" ^ string_of_int index
+
+    fun marker index =
+      Free (marker_name index, HOLogic.natT)
+
+    fun alternative index =
+      let
+        val value = Free ("cycle3_match_value", HOLogic.natT)
+        val predicate =
+          Term.lambda value
+            (URust_Elab_Terms.literal
+              (HOLogic.mk_eq (value, marker index)))
+      in
+        URust_Elab_Terms.matcher_test predicate
+      end
+
+    fun choices [matcher] = matcher
+      | choices (matcher :: matchers) =
+          URust_Elab_Terms.matcher_choice
+            matcher (choices matchers)
+      | choices [] = raise Match
+
+    fun source_term alternatives =
+      let
+        val subject =
+          Free ("cycle3_normalization_subject", HOLogic.natT)
+        val payload =
+          Free ("cycle3_normalization_payload", HOLogic.natT)
+        val success =
+          Term.lambda payload
+            (URust_Elab_Terms.literal payload)
+        val failure =
+          URust_Elab_Terms.literal
+            (HOLogic.mk_number HOLogic.natT 0)
+        val raw =
+          URust_Elab_Terms.matcher_run_value
+            (choices
+              (map alternative (0 upto alternatives - 1)))
+            subject success failure
+      in
+        Syntax.check_term context
+          (Type.constraint expression_type raw)
+      end
+
+    fun occurrences name term =
+      Term.fold_aterms
+        (fn Free (candidate, _) =>
+              if candidate = name then Integer.add 1 else I
+          | _ => I)
+        term 0
+
+    fun check_markers alternatives term =
+      List.app
+        (fn index =>
+          audit_assert
+            ("source marker " ^ string_of_int index ^
+              " does not occur exactly once")
+            (occurrences (marker_name index) term = 1))
+        (0 upto alternatives - 1)
+
+    fun measure alternatives =
+      let
+        val source = source_term alternatives
+        val target =
+          Free ("cycle3_normalized_target", expression_type)
+        val goal =
+          HOLogic.mk_Trueprop
+            (HOLogic.mk_eq (source, target))
+        val _ = check_markers alternatives goal
+        val equation =
+          with_recorded_proofs
+            (fn () =>
+              URust_Matcher_Normalize.normalize_conversion
+                context (Thm.cterm_of context goal))
+        val normalized =
+          Thm.term_of (Thm.rhs_of equation)
+        val _ = check_markers alternatives normalized
+      in
+        {alternatives = alternatives,
+         input = Term.size_of_term goal,
+         normalized = Term.size_of_term normalized,
+         proof = proof_nodes (Thm.proof_of equation)}
+      end
+
+    val measurements =
+      map measure [32, 64, 128]
+
+    fun within_three
+        ({input = input_a, normalized = normalized_a,
+          proof = proof_a, ...},
+         {input = input_b, normalized = normalized_b,
+          proof = proof_b, ...}) =
+      input_b <= 3 * input_a andalso
+      normalized_b <= 3 * normalized_a andalso
+      proof_b <= 3 * proof_a
+
+    val _ =
+      audit_assert "32-to-64 growth exceeded 3x"
+        (within_three
+          (nth measurements 0, nth measurements 1))
+    val _ =
+      audit_assert "64-to-128 growth exceeded 3x"
+        (within_three
+          (nth measurements 1, nth measurements 2))
+
+    fun report
+        {alternatives, input, normalized, proof} =
+      writeln
+        ("Cycle 3 normalization " ^
+          string_of_int alternatives ^
+          ": input=" ^ string_of_int input ^
+          ", normalized=" ^ string_of_int normalized ^
+          ", proof=" ^ string_of_int proof)
+  in
+    val _ = List.app report measurements
+  end
+\<close>
 
 ML_val\<open>
   local
